introduce and prove invaraint LearnedValuesValid

networkInvariantPrototypes/paxos/monotonic/applicationProof.dfy
@@ -19,7 +19,7 @@ predicate ApplicationInv(c: Constants, v: Variables)
   requires v.WF(c)
   requires MessageInv(c, v)
 {
-  && true
+  && LearnedValuesValid(c, v)
 }
 
 predicate Inv(c: Constants, v: Variables)
@@ -29,6 +29,20 @@ predicate Inv(c: Constants, v: Variables)
   && Agreement(c, v)
 }
 
+
+// Analogous to LearnMsgsValid in non-monotonic land
+predicate LearnedValuesValid(c: Constants, v: Variables) 
+  requires v.WF(c)
+{
+  forall idx, vb | 
+    && c.ValidLearnerIdx(idx)
+    && v.learners[idx].Learned(vb)
+  ::
+    && vb in v.learners[idx].receivedAccepts
+    && (exists i ::  
+        && 0 <= i < |v.learners[idx].receivedAccepts[vb]|
+        && |v.learners[idx].receivedAccepts[vb][i]| >= c.f+1)
+}
 
 /***************************************************************************************
 *                                Top-level Obligations                                 *
@@ -51,7 +65,8 @@ lemma InvInductive(c: Constants, v: Variables, v': Variables)
   ensures Inv(c, v')
 {
   MessageInvInductive(c, v, v');
-  assume false;
+  InvNextLearnedValuesValid(c, v, v');
+  assume Agreement(c, v');
 }
 
 
@@ -62,10 +77,80 @@ lemma InvInductive(c: Constants, v: Variables, v': Variables)
 
 
 
+lemma InvNextLearnedValuesValid(c: Constants, v: Variables, v': Variables) 
+  requires Inv(c, v)
+  requires Next(c, v, v')
+  ensures LearnedValuesValid(c, v')
+{
+  forall idx, vb | 
+    && c.ValidLearnerIdx(idx)
+    && v'.learners[idx].Learned(vb)
+  ensures
+    && vb in v'.learners[idx].receivedAccepts
+    && (exists i ::  
+        && 0 <= i < |v'.learners[idx].receivedAccepts[vb]|
+        && |v'.learners[idx].receivedAccepts[vb][i]| >= c.f+1)
+  {
+    var dsStep :| NextStep(c, v, v', dsStep);
+    var actor, msgOps := dsStep.actor, dsStep.msgOps;
+    if && dsStep.LearnerStep? 
+       && idx == actor
+    {
+      var lc, l, l' := c.learnerConstants[actor], v.learners[actor], v'.learners[actor];
+      var step :| LearnerHost.NextStep(lc, l, l', step, msgOps);
+      if step.LearnStep? {
+        var i := |v'.learners[idx].receivedAccepts[vb]| - 1;
+        assert |v'.learners[idx].receivedAccepts[vb][i]| >= c.f+1;  // trigger
+      } else if step.ReceiveStep? && msgOps.recv.value.Accept? {
+        // witness and trigger
+        var i :| 0 <= i < |l.receivedAccepts[vb]| && |l.receivedAccepts[vb][i]| >= c.f+1;
+        assert 0 <= i < |l'.receivedAccepts[vb]| && |l'.receivedAccepts[vb][i]| >= c.f+1;
+      }
+    }
+  }
+}
+
 /***************************************************************************************
 *                            Helper Definitions and Lemmas                             *
 ***************************************************************************************/
 
+// Lemma: For any Learner that learned a Value, that learned value must have been chosen
+lemma LearnedImpliesChosen(c: Constants, v: Variables, idx: LearnerId, vb: ValBal)
+  requires v.WF(c)
+  requires MessageInv(c, v)
+  requires LearnedValuesValid(c, v)
+  requires c.ValidLearnerIdx(idx)
+  requires v.learners[idx].Learned(vb)
+  ensures Chosen(c, v, vb)
+{
+  /* Suppose Learner l learned vb. Then it has a quorum of supporting acceptors for vb in 
+  * l.receivedAccepts, by LearnedValuesValid. By LearnerValidReceivedAccepts, there is a quorum of accept messages
+  * in the network supporting vb. By ValidAcceptMessage, this means there is a quorum of 
+  * acceptors that accepted vb */
+  var l := v.learners[idx];
+
+  // assert vb in l.receivedAccepts;
+
+  assume false;
+  assert Chosen(c, v, vb);
+}
+
+// A quorum of Acceptors accepted the same vb
+predicate Chosen(c: Constants, v: Variables, vb: ValBal) 
+  requires v.WF(c)
+{
+  exists quorum :: IsAcceptorQuorum(c, v, quorum, vb)
+}
+
+predicate IsAcceptorQuorum(c: Constants, v: Variables, aset: set<AcceptorId>, vb: ValBal) 
+  requires v.WF(c)
+{
+  && |aset| >= c.f+1
+  && (forall id | id in aset :: 
+      && c.ValidAcceptorIdx(id)
+      && v.acceptors[id].HasAccepted(vb)
+  )
+}
 
 }  // end module PaxosProof
 
